RocqOfRust/revm/revm_primitives/links/lib.v
@@ -5,6 +5,17 @@ Require Import alloy_primitives.links.aliases.
 Require Import revm.revm_primitives.constants.
 Require Import revm.revm_primitives.lib.
 
+(* pub const BLOCK_HASH_HISTORY: u64 *)
+Instance run_BLOCK_HASH_HISTORY :
+  Run.Trait
+    constants.value_BLOCK_HASH_HISTORY [] [] []
+    ('* u64).
+Proof.
+  constructor.
+  run_symbolic.
+Defined.
+Global Opaque run_BLOCK_HASH_HISTORY.
+
 (* pub const KECCAK_EMPTY: B256 *)
 Instance run_KECCAK_EMPTY :
   Run.Trait
